LeanLinq.lean
@@ -13,5 +13,5 @@ import LeanLinq.Compiler.Expr
 import LeanLinq.Compiler.Query
 import LeanLinq.Statements
 import LeanLinq.Eval.Statements
-import LeanLinq.Fetch
+import LeanLinq.Db
 import LeanLinq.Theorems
